\begin{questions}
    \begin{problem}
    \item[(a)] Let $L$ be a lattice. Show that for any $x, y, z \in L$, we have
    \[ 
    x \vee (y \wedge z) \le (x \vee y) \wedge (x \vee z)
    \]
    \end{problem}

    \begin{solution}
        \begin{proof}
            By definition, we have:
            \[
            \begin{aligned}
                x &\leq x \vee y \\
                x &\leq x \vee z \\
                y \wedge z &\leq y \leq x \vee y \\
                y \wedge z &\leq z \leq x \vee z \\ 
            \end{aligned}
            \]

            which implies that:
            \[
            \begin{aligned}
                x & \leq (x \vee y) \wedge (x\vee z) \\
                y \wedge z & \leq (x \vee y) \wedge (x\vee z)\\
                \implies x \vee (y \wedge z) &\leq (x \vee y) \wedge (x\vee z)\\
            \end{aligned}
            \]
        \end{proof}
    \end{solution}
    \begin{problem}
    \item[(b)] Let $L$ be a finite lattice. We say that $L$ is modular if for any $x, y, z \in L$ we have
    \[
    (x \wedge y) \vee (x \wedge z) = x \wedge (y \vee (x \wedge z)) 
    \]
    
    Show that $L$ is modular if and only if whenever $x \le z$ we have
    \[
    x \vee (y \wedge z) = (x \vee y) \wedge z
    \]
    \end{problem}

    \begin{solution}
        \begin{proof}
            ($\implies$): We have $\forall \; x,y,z \in L$:
            \[
            (x\wedge y)\vee (x\wedge z) = x \wedge (y \vee (x \wedge z))
            \]

            substitute $x$ by $z$ and substitute $z$ by $x$ (switching the position of $x$ and $z$), we have:
            \[
            (z\wedge y) \vee (x \wedge z) = z \wedge (y \vee (x \wedge z))
            \]

            Notice that if $x \leq z \implies x \wedge z = x, \; x \vee z = z$, then substitute such two equation in, we have:
            \[
            x\vee (y\wedge z) = (x \vee y) \wedge z
            \]
            ($\impliedby$): Obviously, we have:
            \[
            x \wedge z  \leq x
            \]

            so substitute into our giving condition we have:
            \[
            \begin{aligned}
            (x\wedge z) \vee (x\wedge y) &= (y\vee (x\wedge z)) \wedge x \\
             \iff (x\wedge y) \vee (x \wedge z) &= x \wedge (y \vee (x \wedge z))
            \end{aligned}
            \]

            which is intended.
        \end{proof}
    \end{solution}
\end{questions}